thys/Transition_Systems_and_Automata/Automata/BA_Translate.thy
@@ -53,9 +53,8 @@ begin
           (\<lambda> x. the (f x)) ` succ A a p,
           acceptinge = (\<lambda> x. the (f x)) ` {p \<in> N. accepting A p}, \<dots> = ba.more A \<rparr>
       }) \<in> ?R"
-    by autoref
-
-  concrete_definition to_baei_impl uses to_baei_impl[unfolded bind_to_let_conv push_in_let_conv]
+    by (autoref_monadic (plain))
+  concrete_definition to_baei_impl uses to_baei_impl
   lemma to_baei_impl_refine'':
     fixes S :: "('statei \<times> 'state) set"
     assumes "finite (nodes A)"
